src/hls/HTLgen.v
@@ -28,6 +28,7 @@ Require Import compcert.backend.RTL.
 
 Require Import vericert.common.Statemonad.
 Require Import vericert.common.Vericertlib.
+Require Import vericert.common.Maps.
 Require Import vericert.hls.AssocMap.
 Require Import vericert.hls.HTL.
 Require Import vericert.hls.ValueInt.
@@ -651,6 +652,218 @@ Definition transl_program (p: RTL.program) : Errors.res HTL.program :=
                                          else transl_main_fundef f)
                              (fun i v => Errors.OK v) p.
 *)
+
+Record renumber_state: Type :=
+  mk_renumber_state {
+    renumber_freshreg : reg;
+    renumber_regmap : PTree.t reg;
+    renumber_clk : reg;
+  }.
+
+Module RenumberState <: State.
+  Definition st := renumber_state.
+
+  Definition st_prop (st1 st2 : st) := renumber_clk st1 = renumber_clk st2.
+
+  Lemma st_refl : forall (s : st), st_prop s s.
+  Proof. constructor. Qed.
+
+  Lemma st_trans : forall s1 s2 s3, st_prop s1 s2 -> st_prop s2 s3 -> st_prop s1 s3.
+  Proof. congruence. Qed.
+End RenumberState.
+
+Module RenumberMonad := Statemonad(RenumberState).
+Module RenumberMonadExtra := Monad.MonadExtra(RenumberMonad).
+
+Section RENUMBER.
+  Import RenumberMonad.
+  Import RenumberState.
+  Import RenumberMonadExtra.
+  Import MonadNotation.
+
+  Program Definition map_reg (r: reg) : mon reg :=
+    fun st => OK
+         (renumber_freshreg st)
+         (mk_renumber_state (Pos.succ (renumber_freshreg st))
+                            (PTree.set r (renumber_freshreg st) (renumber_regmap st))
+                            (renumber_clk st))
+         _.
+  Next Obligation. unfold st_prop; auto. Qed.
+
+  Program Definition clear_mapping : mon unit :=
+    fun st => OK
+         tt
+         (mk_renumber_state (renumber_freshreg st)
+                            (PTree.empty reg)
+                            (renumber_clk st))
+         _.
+  Next Obligation. unfold st_prop; auto. Qed.
+
+  Definition renumber_reg (r : reg) : mon reg :=
+    do st <- get;
+    match PTree.get r (renumber_regmap st) with
+    | Some reg' => ret reg'
+    | None => map_reg r
+    end.
+
+  Definition get_clk : mon reg := do st <- get; ret (renumber_clk st).
+
+  Fixpoint renumber_expr (expr : Verilog.expr) :=
+    match expr with
+    | Vlit val => ret (Vlit val)
+    | Vvar reg =>
+      do reg' <- renumber_reg reg;
+      ret (Vvar reg')
+    | Vvari reg e =>
+      do reg' <- renumber_reg reg;
+      do e' <- renumber_expr e;
+      ret (Vvari reg' e')
+    | Vinputvar reg =>
+      do reg' <- renumber_reg reg;
+      ret (Vvar reg')
+    | Vbinop op e1 e2 =>
+      do e1' <- renumber_expr e1;
+      do e2' <- renumber_expr e2;
+      ret (Vbinop op e1' e2')
+    | Vunop op e =>
+      do e' <- renumber_expr e;
+      ret (Vunop op e')
+    | Vternary e1 e2 e3 =>
+      do e1' <- renumber_expr e1;
+      do e2' <- renumber_expr e2;
+      do e3' <- renumber_expr e3;
+      ret (Vternary e1' e2' e3')
+    | Vrange r e1 e2 =>
+      do e1' <- renumber_expr e1;
+      do e2' <- renumber_expr e2;
+      do r' <- renumber_reg r;
+      ret (Vrange r e1' e2')
+    end.
+
+  Fixpoint renumber_stmnt (stmnt : Verilog.stmnt) :=
+    match stmnt with
+    | Vskip => ret Vskip
+    | Vseq s1 s2 =>
+      do s1' <- renumber_stmnt s1;
+      do s2' <- renumber_stmnt s2;
+      ret (Vseq s1' s2')
+    | Vcond e s1 s2 =>
+      do e' <- renumber_expr e;
+      do s1' <- renumber_stmnt s1;
+      do s2' <- renumber_stmnt s2;
+      ret (Vcond e' s1' s2')
+    | Vcase e cs def =>
+      do e' <- renumber_expr e;
+      do cs' <- sequence (map
+                       (fun (c : (Verilog.expr * Verilog.stmnt)) =>
+                      let (c_expr, c_stmnt) := c in
+                      do expr' <- renumber_expr c_expr;
+                      do stmnt' <- renumber_stmnt c_stmnt;
+                      ret (expr', stmnt')) cs);
+      do def' <- match def with
+                | None => ret None
+                | Some d => do def' <- renumber_stmnt d; ret (Some def')
+                end;
+      ret (Vcase e' cs' def')
+    | Vblock e1 e2 =>
+      do e1' <- renumber_expr e1;
+      do e2' <- renumber_expr e2;
+      ret (Vblock e1' e2')
+    | Vnonblock e1 e2 =>
+      do e1' <- renumber_expr e1;
+      do e2' <- renumber_expr e2;
+      ret (Vnonblock e1' e2')
+    end.
+
+  Definition renumber_module (m : HTL.module) : mon HTL.module :=
+      do mod_start' <- renumber_reg (HTL.mod_start m);
+      do mod_reset' <- renumber_reg (HTL.mod_reset m);
+      do mod_clk' <- get_clk;
+      do mod_finish' <- renumber_reg (HTL.mod_finish m);
+      do mod_return' <- renumber_reg (HTL.mod_return m);
+      do mod_st' <- renumber_reg (HTL.mod_st m);
+      do mod_stk' <- renumber_reg (HTL.mod_stk m);
+      do mod_params' <- traverselist renumber_reg (HTL.mod_params m);
+      do mod_controllogic' <- traverse_ptree1 renumber_stmnt (HTL.mod_controllogic m);
+      do mod_datapath' <- traverse_ptree1 renumber_stmnt (HTL.mod_datapath m);
+
+      do _ <- clear_mapping;
+
+      match zle (Z.pos (max_pc_map mod_datapath')) Integers.Int.max_unsigned,
+            zle (Z.pos (max_pc_map mod_controllogic')) Integers.Int.max_unsigned with
+      | left LEDATA, left LECTRL =>
+        ret (HTL.mkmodule
+           mod_params'
+           mod_datapath'
+           mod_controllogic'
+           (HTL.mod_entrypoint m)
+           mod_st'
+           (HTL.mod_stk m)
+           (HTL.mod_stk_len m)
+           mod_finish'
+           mod_return'
+           mod_start'
+           mod_reset'
+           mod_clk'
+           (HTL.mod_scldecls m)
+           (HTL.mod_arrdecls m)
+           (HTL.mod_externctrl m)
+           (conj (max_pc_wf _ _ LECTRL) (max_pc_wf _ _ LEDATA)))
+      | _, _ => error (Errors.msg "More than 2^32 states.")
+      end.
+
+  Definition renumber_fundef (fundef : HTL.fundef) : mon HTL.fundef :=
+    match fundef with
+    | Internal m => do renumbered <- renumber_module m; ret (Internal renumbered)
+    | _ => ret fundef
+    end.
+
+  Section TRANSF_PROGRAM_STATEFUL.
+    Import RenumberMonad.
+    Import RenumberState.
+    Import RenumberMonadExtra.
+    Import MonadNotation.
+
+    Variables A B V : Type.
+    Variable transf_fun: ident -> A -> RenumberMonad.mon B.
+
+    Fixpoint transf_globdefs (l: list (ident * globdef A V)) : RenumberMonad.mon (list (ident * globdef B V)) :=
+      match l with
+      | nil => RenumberMonad.ret nil
+      | (id, Gfun f) :: l' =>
+        do tf <- transf_fun id f;
+        do tl' <- transf_globdefs l';
+        RenumberMonad.ret ((id, Gfun tf) :: tl')
+      | (id, Gvar v) :: l' =>
+        do tl' <- transf_globdefs l';
+        RenumberMonad.ret ((id, Gvar v) :: tl')
+      end.
+
+    Definition transform_stateful_program (init_state : RenumberState.st) (p: AST.program A V) : Errors.res (AST.program B V) :=
+      RenumberMonad.run_mon init_state (
+                          do gl' <- transf_globdefs p.(prog_defs);
+                          RenumberMonad.ret (mkprogram gl' p.(prog_public) p.(prog_main))).
+
+  End TRANSF_PROGRAM_STATEFUL.
+
+  Definition get_main_clk (p : HTL.program) : Errors.res reg :=
+    let ge := Globalenvs.Genv.globalenv p in
+    match Globalenvs.Genv.find_symbol ge p.(AST.prog_main) with
+    | Some b =>
+      match Globalenvs.Genv.find_funct_ptr ge b with
+      | Some (AST.Internal m) => Errors.OK (HTL.mod_clk m)
+      | _ => Errors.Error (Errors.msg "Cannot find internal main for renumbering")
+      end
+    | _ => Errors.Error (Errors.msg "Cannot find internal main for renumbering")
+    end.
+
+  Definition renumber_program (p : HTL.program) : Errors.res HTL.program :=
+    Errors.bind (get_main_clk p)
+                (fun main_clk => transform_stateful_program _ _ _
+                                                         (fun _ => renumber_fundef)
+                                                         (mk_renumber_state 1%positive (PTree.empty reg) main_clk)
+                                                         p).
+End RENUMBER.
 
 Definition main_is_internal (p : RTL.program) : bool :=
   let ge := Globalenvs.Genv.globalenv p in
